Minor2

Kura/Operation/Map.lean
@@ -1,4 +1,5 @@
 import Kura.Subgraph
+import Kura.Dep.Finset
 
 
 open Set Function
@@ -18,29 +19,53 @@ namespace Graph
 --     obtain ⟨v, hv, rfl⟩ := h
 --     use v, hv.vx_mem)
 
-/-- Map `G : Graph α β` to a `Graph α' β` with the same edge set
-by applying a function `f : α → α'` to each vertex.
-Edges between identified vertices become loops. -/
-@[simps]
-def vxMap {α' : Type*} (G : Graph α β) (f : α → α') : Graph α' β where
-  V := f '' G.V
-  E := G.E
-  Inc₂ e x' y' := ∃ x y, G.Inc₂ e x y ∧ x' = f x ∧ y' = f y
-  inc₂_symm := by
-    rintro e - - ⟨x, y, h, rfl, rfl⟩
-    exact ⟨y, x, h.symm, rfl, rfl⟩
-  eq_or_eq_of_inc₂_of_inc₂ := by
-    rintro e - - - - ⟨x, y, hxy, rfl, rfl⟩ ⟨z, w, hzw, rfl, rfl⟩
-    obtain rfl | rfl := hxy.left_eq_or_eq_of_inc₂ hzw <;> simp
-  edge_mem_iff_exists_inc₂ e := by
-    refine ⟨fun h ↦ ?_, ?_⟩
-    · obtain ⟨x, y, hxy⟩ := exists_inc₂_of_mem_edgeSet h
-      exact ⟨_, _, _, _, hxy, rfl, rfl⟩
-    rintro ⟨-, -, x, y, h, rfl, rfl⟩
-    exact h.edge_mem
-  vx_mem_left_of_inc₂ := by
-    rintro e - - ⟨x, y, h, rfl, rfl⟩
-    exact Set.mem_image_of_mem _ h.vx_mem_left
+-- /-- Map `G : Graph α β` to a `Graph α' β` with the same edge set
+-- by applying a function `f : α → α'` to each vertex.
+-- Edges between identified vertices become loops. -/
+-- @[simps]
+-- def vxMap {α' : Type*} (G : Graph α β) (f : α → α') : Graph α' β where
+--   V := f '' G.V
+--   E := G.E
+--   Inc₂ e x' y' := ∃ x y, G.Inc₂ e x y ∧ x' = f x ∧ y' = f y
+--   inc₂_symm := by
+--     rintro e - - ⟨x, y, h, rfl, rfl⟩
+--     exact ⟨y, x, h.symm, rfl, rfl⟩
+--   eq_or_eq_of_inc₂_of_inc₂ := by
+--     rintro e - - - - ⟨x, y, hxy, rfl, rfl⟩ ⟨z, w, hzw, rfl, rfl⟩
+--     obtain rfl | rfl := hxy.left_eq_or_eq_of_inc₂ hzw <;> simp
+--   edge_mem_iff_exists_inc₂ e := by
+--     refine ⟨fun h ↦ ?_, ?_⟩
+--     · obtain ⟨x, y, hxy⟩ := exists_inc₂_of_mem_edgeSet h
+--       exact ⟨_, _, _, _, hxy, rfl, rfl⟩
+--     rintro ⟨-, -, x, y, h, rfl, rfl⟩
+--     exact h.edge_mem
+--   vx_mem_left_of_inc₂ := by
+--     rintro e - - ⟨x, y, h, rfl, rfl⟩
+--     exact Set.mem_image_of_mem _ h.vx_mem_left
+
+@[simps!]
+def vxMap {α' : Type*} (G : Graph α β) (f : α → α') : Graph α' β :=
+  oftoMultiset (f '' G.V) (fun e ↦ (G.toMultiset e).map f) fun e v h ↦ (by
+    simp only [Multiset.mem_map, inc_iff_mem_toMultiset, mem_image] at h ⊢
+    obtain ⟨v, hv, rfl⟩ := h
+    use v, hv.vx_mem)
+
+/-- `vxMap` has the expected incidence predicate. -/
+@[simp]
+lemma vxMap_inc : (G.vxMap φ).Inc e x ↔ ∃ v, G.Inc e v ∧ φ v = x := by
+  rw [← inc_iff_mem_toMultiset]
+  unfold vxMap
+  rw [oftoMultiset_toMultiset (by simp [em])]
+  simp
+
+@[simp]
+lemma vxMap_toMultiset : (G.vxMap φ).toMultiset e = (G.toMultiset e).map φ := by
+  unfold vxMap
+  rw [oftoMultiset_toMultiset (by simp [em])]
+
+@[simp]
+lemma vxMap_inc₂' : (G.vxMap φ).Inc₂ e x y ↔ ∃ v w, G.Inc₂ e v w ∧ φ v = x ∧ φ w = y := by
+  simp_rw [← toMultiset_eq_pair_iff, vxMap_toMultiset, Multiset.map_eq_pair_iff]
 
 def edgePreimg {β' : Type*} (G : Graph α β) (σ : β' → β) : Graph α β' :=
   oftoMultiset G.V (G.toMultiset <| σ ·) (fun e v hv ↦ by
