Kura/Operation/Minor2.lean
@@ -20,66 +20,59 @@ def Setify.HasIsom (G : Graph α β) : G ≤↔ G.Setify :=
 
 lemma Setify.IsPartitionGraph (G : Graph α β) : G.Setify.IsPartitionGraph := by
   use Partition.discrete G.V
-  simp only [Partition.discrete.parts, Setify, vxMap.V]
+  simp only [Partition.discrete.parts, Setify, vxMap_vxSet]
 
+@[simps!]
 def SetContract (G : Graph (Set α) β) (C : Set β) : Graph (Set α) β :=
-  G.vxMap (⋃₀ G{C}.Component ·) \ C
+  G.vxMap (⋃₀ (G ↾ C).Component ·) ＼ C
 
 scoped infix:100 " / " => Graph.SetContract
 
 variable {G : Graph (Set α) β} {C D : Set β}
 
 @[simp]
-lemma SetContract.V : (G / C).V = (⋃₀ G{C}.Component ·) '' G.V := rfl
-
-@[simp]
-lemma SetContract.E : (G / C).E = G.E \ C := by
+lemma setContract_toMultiset (heC : e ∉ C) :
+    (G / C).toMultiset e = (G.toMultiset e).map (⋃₀ (G ↾ C).Component ·) := by
   simp [SetContract]
-
-@[simp]
-lemma SetContract.toMultiset (heC : e ∉ C) :
-    (G / C).toMultiset e = (G.toMultiset e).map (⋃₀ G{C}.Component ·) := by
-  simp [SetContract]
-  rw [← vxMap_toMultiset_eq_map_toMultiset, toMultiset_eq_toMultiset]
+  rw [← vxMap_toMultiset, toMultiset_eq_toMultiset_iff]
   ext x y
   simp [heC]
 
 @[simp]
-lemma SetContract.Inc {u : Set α} :
-    (G / C).Inc e u ↔ e ∉ C ∧ ∃ v, G.Inc e v ∧ ⋃₀ G{C}.Component v = u := by
-  simp only [SetContract, edgeDel_inc, vxMap_inc_iff]
-  tauto
+lemma setContract_inc {u : Set α} :
+    (G / C).Inc e u ↔ e ∉ C ∧ (∃ v, G.Inc e v ∧ ⋃₀ (G ↾ C).Component v = u) := by
+  simp_rw [SetContract, inc_iff_exists_inc₂, edgeDelete_inc₂, exists_and_left,
+    ← inc_iff_exists_inc₂, vxMap_inc]
 
 @[simp]
-lemma SetContract.Inc₂ {u v : Set α} :
-    (G / C).Inc₂ e u v ↔ e ∉ C ∧ ∃ x y, G.Inc₂ e x y ∧ ⋃₀ G{C}.Component x = u ∧ ⋃₀ G{C}.Component y = v := by
-  simp only [SetContract, edgeDel_inc₂, vxMap_inc₂_iff]
-  tauto
+lemma setContract_inc₂ {u v : Set α} :
+    (G / C).Inc₂ e u v ↔ e ∉ C ∧ (∃ x y, G.Inc₂ e x y ∧ ⋃₀ (G ↾ C).Component x = u ∧ ⋃₀ (G ↾ C).Component y = v) := by
+  simp_rw [SetContract, edgeDelete_inc₂, vxMap_inc₂']
 
-lemma SetContract.subset_map (C : Set β) {u : Set α} (hu : u ∈ G.V) : u ⊆ ⋃₀ G{C}.Component u :=
-  subset_sUnion_of_subset (G{C}.Component u) u (fun _ a ↦ a) (Connected.refl hu)
+lemma SetContract.subset_map (C : Set β) {u : Set α} (hu : u ∈ G.V) : u ⊆ ⋃₀ (G ↾ C).Component u :=
+  subset_sUnion_of_subset ((G ↾ C).Component u) u (fun _ a ↦ a) (VxConnected.refl hu)
 
 lemma SetContract.map_eq_iff' {u v : Set α} (hP : G.IsPartitionGraph) (hv : v ∈ G.V) :
-    ⋃₀ G{C}.Component u = ⋃₀ G{C}.Component v ↔ G{C}.Connected u v := by
+    ⋃₀ (G ↾ C).Component u = ⋃₀ (G ↾ C).Component v ↔ (G ↾ C).VxConnected u v := by
   obtain ⟨P, hP⟩ := hP
   rw [← hP] at hv
   constructor <;> intro h
-  · have : v ⊆ ⋃₀ G{C}.Component v := subset_map C (hP ▸ hv)
-    rw [← h, P.subset_sUnion_iff_mem hv (by rw [hP, ← restrict_V (R := C)]; exact Component.subset_V)] at this
+  · have : v ⊆ ⋃₀ (G ↾ C).Component v := subset_map C (hP ▸ hv)
+    rw [← h, P.subset_sUnion_iff_mem hv (by rw [hP, ← edgeRestrict_vxSet]; exact component_subset_V)] at this
     simpa using this
   · ext x
-    simp only [mem_sUnion, Component.mem]
-    have : ∀ t, G{C}.Connected u t ↔ G{C}.Connected v t := fun _ ↦ rel_congr_left h
+    simp only [mem_sUnion, mem_component_iff]
+    have : ∀ t, (G ↾ C).VxConnected u t ↔ (G ↾ C).VxConnected v t := fun _ ↦ rel_congr_left h
     simp_rw [this]
 
 lemma SetContract.map_eq_iff {u v : Set α} (hP : G.IsPartitionGraph) (hu : u ∈ G.V) :
-    ⋃₀ G{C}.Component u = ⋃₀ G{C}.Component v ↔ G{C}.Connected u v := by
-  rw [eq_comm, Connected.comm, SetContract.map_eq_iff' hP hu]
+    ⋃₀ (G ↾ C).Component u = ⋃₀ (G ↾ C).Component v ↔ (G ↾ C).VxConnected u v := by
+  rw [eq_comm, vxConnected_comm, SetContract.map_eq_iff' hP hu]
 
 @[simp]
 lemma SetContract.map_mem_iff {u : Set α} (hP : G.IsPartitionGraph) :
-    (⋃₀ G{C}.Component u) ∈ (G / C).V ↔ u ∈ G.V := by
-  simp only [V, mem_image]
+    (⋃₀ (G ↾ C).Component u) ∈ (G / C).V ↔ u ∈ G.V := by
+  simp only [SetContract_vxSet, mem_image]
   constructor <;> rintro h
   · obtain ⟨x, hx, heq⟩ := h
     rw [map_eq_iff hP hx] at heq
@@ -88,7 +81,7 @@ lemma SetContract.map_mem_iff {u : Set α} (hP : G.IsPartitionGraph) :
 
 -- @[simp]
 -- lemma SetContract.merged_iff {u v : Set α} (hP : G.IsPartitionGraph) (hu : u ∈ G.V) (hv : v ∈ G.V) :
---     (∃ x ∈ (G / C).V, u ⊆ x ∧ v ⊆ x) ↔ G{C}.Connected u v := by
+--     (∃ x ∈ (G / C).V, u ⊆ x ∧ v ⊆ x) ↔ (G ↾ C).Connected u v := by
 --   obtain ⟨P, hP⟩ := hP
 --   constructor
 --   · rintro ⟨x, hx, hux, hvx⟩
@@ -97,104 +90,102 @@ lemma SetContract.map_mem_iff {u : Set α} (hP : G.IsPartitionGraph) :
 --     rw [← hP] at hS hu hv
 --     simp only [Component] at hux hvx
 --     exact ((P.subset_sUnion_iff_mem hu (hP ▸ fun x hx ↦ (by
---       simpa using hx : G{C}.Connected S x).mem_right)).mp hux).symm.trans
+--       simpa using hx : (G ↾ C).Connected S x).mem_right)).mp hux).symm.trans
 --       ((P.subset_sUnion_iff_mem hv (hP ▸ fun x hx ↦ (by
---       simpa using hx : G{C}.Connected S x).mem_right)).mp hvx)
+--       simpa using hx : (G ↾ C).Connected S x).mem_right)).mp hvx)
 --   · intro h
---     use ⋃₀ G{C}.Component u, (by use u), ?_
---     · exact subset_sUnion_of_subset (G{C}.Component u) v (fun ⦃a⦄ a ↦ a) h
---     · exact subset_sUnion_of_subset (G{C}.Component u) u (fun ⦃a⦄ a ↦ a) (Connected.refl hu)
+--     use ⋃₀ (G ↾ C).Component u, (by use u), ?_
+--     · exact subset_sUnion_of_subset ((G ↾ C).Component u) v (fun ⦃a⦄ a ↦ a) h
+--     · exact subset_sUnion_of_subset ((G ↾ C).Component u) u (fun ⦃a⦄ a ↦ a) (Connected.refl hu)
 
 lemma SetContract.IsPartitionGraph (C : Set β) (hP : G.IsPartitionGraph) :
     (G / C).IsPartitionGraph := by
   obtain ⟨P, hP⟩ := hP
-  use G{C}.ConnectedPartition.flatten ⟨P, by simp [hP]⟩
-  simp only [Partition.flatten_parts, sSup_eq_sUnion, ConnectedPartition.parts, ComponentSets,
-    restrict_V, V]
+  use (G ↾ C).ConnectedPartition.flatten ⟨P, by simp [hP]⟩
+  simp only [Partition.flatten_parts, sSup_eq_sUnion, connectedPartition_parts, ComponentSets,
+    edgeRestrict_vxSet, SetContract_vxSet]
   rw [image_image]
 
 lemma setContract_edgeDel_comm (G : Graph (Set α) β) (hCD : Disjoint C D) :
-    (G / C) \ D = (G \ D) / C := by
-  have heq : G{C} = (G \ D){C} := by
-    rw [edgeDel, restrict_restrict_eq_restrict_inter, restrict_eq_restrict_iff]
+    (G / C) ＼ D = (G ＼ D) / C := by
+  have heq : (G ↾ C) = (G ＼ D) ↾ C := by
+    rw [edgeDelete_eq_edgeRestrict, edgeRestrict_edgeRestrict, edgeRestrict_eq_edgeRestrict_iff]
     tauto_set
-  refine ext_inc₂ ?_ fun e x y ↦ ?_
+  refine ext_inc ?_ fun e x ↦ ?_
   · ext u
-    simp only [edgeDel_V, SetContract.V, mem_image, heq]
-  · simp only [edgeDel_inc₂, SetContract.Inc₂, ← heq]
+    simp only [edgeDelete_vxSet, SetContract_vxSet, heq, mem_image]
+  · simp only [edgeDelete_inc, setContract_inc, ← heq]
     tauto
 
 lemma SetContract.foo {u v : Set α} (hP : G.IsPartitionGraph)
-    (hTconn : (G / C){D}.Connected (⋃₀ G{C}.Component v) (⋃₀ G{C}.Component u)) :
-    G{C ∪ D}.Connected v u := by
+    (hTconn : (G / C ↾ D).VxConnected (⋃₀ (G ↾ C).Component v) (⋃₀ (G ↾ C).Component u)) :
+    (G ↾ (C ∪ D)).VxConnected v u := by
   have hu : u ∈ G.V := (SetContract.map_mem_iff hP).mp hTconn.mem_right
   have hv : v ∈ G.V := (SetContract.map_mem_iff hP).mp hTconn.mem_left
-  obtain ⟨w, hwVd, hwfst, hwlst⟩ := connected_iff_exists_walk.mp hTconn ; clear hTconn
+  obtain ⟨w, hwVd, hwfst, hwlst⟩ := vxConnected_iff_exists_walk.mp hTconn ; clear hTconn
   induction w generalizing v with
   | nil v =>
     simp only [WList.nil_first, WList.nil_last] at hwfst hwlst
     rw [hwfst, map_eq_iff' hP hu] at hwlst
-    exact hwlst.of_le (restrict_mono G subset_union_left)
+    exact hwlst.of_le (edgeRestrict_mono_right G subset_union_left)
   | cons a e w ih =>
-    simp only [WList.first_cons, WList.last_cons, cons_isWalk_iff, restrict_inc₂_iff,
-      Inc₂] at hwfst hwlst hwVd
-    obtain ⟨⟨⟨heC, x, y, hbtw, rfl, hy⟩, heD⟩, hwVd⟩ := hwVd
+    simp only [WList.first_cons, WList.last_cons, cons_isWalk_iff, edgeRestrict_inc₂,
+      setContract_inc₂] at hwfst hwlst hwVd
+    obtain ⟨⟨heD, heC, x, y, hbtw, rfl, hy⟩, hwVd⟩ := hwVd
     rw [map_eq_iff' hP hv] at hwfst
-    exact hwfst.symm.of_le (restrict_mono G subset_union_left)
-    |>.trans (restrict_inc₂_iff.mpr ⟨hbtw, by tauto⟩).connected
+    exact hwfst.symm.of_le (edgeRestrict_mono_right G subset_union_left)
+    |>.trans ((edgeRestrict_inc₂ _ _ _ _ _).mpr ⟨by tauto, hbtw⟩).vxConnected
     |>.trans (ih hbtw.vx_mem_right hwVd hy.symm hwlst)
 
-lemma SetContract.foo2 {u v : Set α} (hP : G.IsPartitionGraph) (h : G{C ∪ D}.Connected v u) :
-    (G / C){D}.Connected (⋃₀ G{C}.Component v) (⋃₀ G{C}.Component u) := by
-  obtain ⟨w, hwVd, rfl, rfl⟩ := connected_iff_exists_walk.mp h ; clear h
+lemma SetContract.foo2 {u v : Set α} (hP : G.IsPartitionGraph) (h : (G ↾ (C ∪ D)).VxConnected v u) :
+    (G / C ↾ D).VxConnected (⋃₀ (G ↾ C).Component v) (⋃₀ (G ↾ C).Component u) := by
+  obtain ⟨w, hwVd, rfl, rfl⟩ := vxConnected_iff_exists_walk.mp h ; clear h
   induction w with
   | nil x =>
-    simp only [WList.nil_last, WList.nil_first, Connected.refl_iff, restrict_V, V,
+    simp only [WList.nil_last, WList.nil_first, vxConnected_self, edgeRestrict_vxSet, V,
       mem_image]
     use x, by simpa using hwVd
   | cons a e w ih =>
-    simp only [cons_isWalk_iff, restrict_inc₂_iff, mem_union, WList.last_cons,
+    simp only [cons_isWalk_iff, edgeRestrict_inc₂, mem_union, WList.last_cons,
       WList.first_cons] at hwVd ⊢
-    obtain ⟨⟨hbtw, he⟩, hwVd⟩ := hwVd
-    by_cases heC : e ∈ C <;> refine Connected.trans ?_ (ih hwVd)
-    · convert Connected.refl ?_ using 1
+    obtain ⟨⟨he, hbtw⟩, hwVd⟩ := hwVd
+    by_cases heC : e ∈ C <;> refine VxConnected.trans ?_ (ih hwVd)
+    · convert VxConnected.refl ?_ using 1
       · rw [map_eq_iff' hP hbtw.vx_mem_left]
-        exact (restrict_inc₂_iff.mpr ⟨hbtw.symm, heC⟩).connected
+        exact ((edgeRestrict_inc₂ _ _ _ _ _).mpr ⟨heC, hbtw.symm⟩).vxConnected
       · use a, hbtw.vx_mem_left
     · simp only [heC, false_or] at he
-      refine Inc₂.connected ?_ (e := e)
-      simp only [restrict_inc₂_iff, Inc₂, heC, not_false_eq_true, true_and, he, and_true]
+      refine Inc₂.vxConnected ?_ (e := e)
+      simp only [edgeRestrict_inc₂, he, setContract_inc₂, heC, not_false_eq_true, true_and]
       use a, w.first
 
 lemma SetContract.map_map (C D : Set β) (hP : G.IsPartitionGraph) {v : Set α}  :
-    ⋃₀ (G / C){D}.Component (⋃₀ G{C}.Component v) = ⋃₀ G{C ∪ D}.Component v := by
+    ⋃₀ (G / C ↾ D).Component (⋃₀ (G ↾ C).Component v) = ⋃₀ (G ↾ (C ∪ D)).Component v := by
   ext x
-  simp only [mem_sUnion, Component.mem]
+  simp only [mem_sUnion, mem_component_iff]
   constructor
   · rintro ⟨T, hTconn, hxT⟩
     obtain ⟨u, hu, rfl⟩ := hTconn.mem_right
     obtain ⟨u', hu'conn, hxu'⟩ := hxT
-    use u', (foo hP hTconn).trans (hu'conn.of_le (restrict_mono G subset_union_left))
+    use u', (foo hP hTconn).trans (hu'conn.of_le (edgeRestrict_mono_right G subset_union_left))
   · rintro ⟨u, huconn, hxu⟩
-    use ⋃₀ G{C}.Component u, foo2 hP huconn
+    use ⋃₀ (G ↾ C).Component u, foo2 hP huconn
     refine subset_map C ?_ hxu
     exact huconn.mem_right
 
 lemma SetContract.contract_contract (C D : Set β) (hP : G.IsPartitionGraph) :
     (G / C) / D = G / (C ∪ D) := by
-  refine ext_inc₂ ?_ fun e x y ↦ ?_
+  refine Graph.ext ?_ fun e x y ↦ ?_
   · ext u
-    simp only [V, mem_image, exists_exists_and_eq_and, map_map C D hP]
-  · simp only [Inc₂, mem_union, not_or]
+    simp only [SetContract_vxSet, mem_image, exists_exists_and_eq_and, map_map C D hP]
+  · simp only [setContract_inc₂, mem_union, not_or]
     constructor
     · rintro ⟨heD, _, _, ⟨heC, x, y, hbtw, rfl, rfl⟩, rfl, rfl⟩
       simp only [heC, not_false_eq_true, heD, and_self, map_map C D hP, true_and]
       use x, y
     · rintro ⟨⟨heC, heD⟩, x, y, hbtw, rfl, rfl⟩
       simp only [heD, not_false_eq_true, heC, true_and]
-      use ⋃₀ G{C}.Component x, ⋃₀ G{C}.Component y, (by use x, y), map_map C D hP, map_map C D hP
-
-
+      use ⋃₀ (G ↾ C).Component x, ⋃₀ (G ↾ C).Component y, (by use x, y), map_map C D hP, map_map C D hP
 
 
 end Graph
